Refine InterleaveLists definition

theories/InterleaveLists.v
@@ -12,13 +12,13 @@ Let L := list T.
 
 (* This datastructure reflects a _permutation_ that is needed to
 interleave lists: *)
-Inductive InterleaveLists (l r : L) : L -> Prop :=
+Inductive InterleaveLists (l : L) : L -> Prop :=
 | intl_orig :
-    InterleaveLists l r (l ++ r)
+    InterleaveLists l l
 | intl_shuf : forall l' r' a b,
-    InterleaveLists l r (l' ++ a :: b :: r') ->
+    InterleaveLists l (l' ++ a :: b :: r') ->
     commute a b ->
-    InterleaveLists l r (l' ++ b :: a :: r').
+    InterleaveLists l (l' ++ b :: a :: r').
 
 (* TODO: Prove completeness of this defintion *)
 
@@ -28,16 +28,10 @@ Section tests.
 
 Let comm a b := odd a /\ even b.
 
-Example example_interleaved_list_1 : InterleaveLists comm [] [] [].
+Example example_interleaved_list_1 : InterleaveLists comm [] [].
 Proof. constructor; auto. Qed.
 
-Example example_interleaved_list_2 : InterleaveLists comm [1; 3] [2; 4] [1; 3; 2; 4].
-Proof.
-  replace [1; 3; 2; 4] with ([1; 3] ++ [2; 4]) by auto.
-  constructor.
-Qed.
-
-Example example_interleaved_list_3 : InterleaveLists comm [1; 3] [2; 4] [1; 2; 3; 4].
+Example example_interleaved_list_3 : InterleaveLists comm [1; 3; 2; 4] [1; 2; 3; 4].
 Proof.
   replace [1; 2; 3; 4] with ([1] ++ 2 :: 3 :: [4]) by auto.
   constructor.
